theories/Control/State.v
@@ -18,7 +18,7 @@ Local Open Scope free_weq_scope.
 Definition StateT
            (s: Type)
            (m: Type -> Type)
-           `{Monad m}
+          `{Monad m}
            (a: Type)
   : Type :=
   s -> m (a * s).
@@ -84,104 +84,7 @@ Definition state_map
            (fs:  StateT s m a)
   : StateT s m b :=
     fun s
-    => o <- fs s                                                     ;
-       pure (f (fst o), (snd o)).
-
-Definition statet_weq
-           {m: Type -> Type}
-          `{Monad m}
-           {s:   Type}
-          `{WEq s}
-           {a: Type}
-          `{WEq a}
-           (p g: StateT s m a)
-  : Prop :=
-  forall (x: s),
-    fst <$> p x == fst <$> g x
-    /\ snd <$> p x == snd <$> g x.
-
-Lemma statet_weq_refl
-      {m: Type -> Type}
-     `{Monad m}
-      {s:   Type}
-     `{WEq s}
-      {a: Type}
-     `{WEq a}
-      (p: StateT s m a)
-  : statet_weq p p.
-Proof.
-  split.
-  + reflexivity.
-  + reflexivity.
-Qed.
-
-Lemma statet_weq_sym
-      {m: Type -> Type}
-     `{Monad m}
-      {s:   Type}
-     `{WEq s}
-      {a: Type}
-     `{WEq a}
-      (p q: StateT s m a)
-  : statet_weq p q
-    -> statet_weq q p.
-Proof.
-  intros G x.
-  assert (G': fst <$> p x == fst <$> q x /\ snd <$> p x == snd <$> q x)
-    by exact (G x).
-  destruct G' as [G1 G2].
-  split; symmetry; [ exact G1
-                   | exact G2
-                   ].
-Qed.
-
-Lemma statet_weq_trans
-      {m: Type -> Type}
-     `{Monad m}
-      {s:   Type}
-     `{WEq s}
-      {a: Type}
-     `{WEq a}
-      (p q r: StateT s m a)
-  : statet_weq p q
-    -> statet_weq q r
-    -> statet_weq p r.
-Proof.
-  intros Q R x.
-  assert (Q': fst <$> p x == fst <$> q x /\ snd <$> p x == snd <$> q x)
-    by exact (Q x).
-  assert (R': fst <$> q x == fst <$> r x /\ snd <$> q x == snd <$> r x)
-    by exact (R x).
-  destruct Q' as [Q1 Q2].
-  destruct R' as [R1 R2].
-  split.
-  + rewrite Q1; exact R1.
-  + rewrite Q2; exact R2.
-Qed.
-
-Add Parametric Relation
-    (m: Type -> Type)
-   `{Monad m}
-    (s:   Type)
-   `{WEq s}
-    (a: Type)
-   `{WEq a}
-  : (StateT s m a) (statet_weq)
-    reflexivity proved by statet_weq_refl
-    symmetry proved by statet_weq_sym
-    transitivity proved by statet_weq_trans
-      as statet_weq_equiv.
-
-Instance statet_WEq
-         (m: Type -> Type)
-        `{Monad m}
-         (s:   Type)
-        `{WEq s}
-         (a: Type)
-        `{WEq a}
-  : WEq (StateT s m a) :=
-  { weq := statet_weq
-  }.
+    => (fun o => (f (fst o), snd o)) <$> fs s.
 
 Lemma state_functor_identity
       (m: Type -> Type)
@@ -193,10 +96,16 @@ Lemma state_functor_identity
       (ps: StateT s m a)
   : state_map _ _ id ps == id ps.
 Proof.
-  constructor.
-  + unfold state_map.
-    unfold id.
-Admitted.
+  cbn.
+  unfold function_weq, state_map.
+  intros x.
+  assert (R1: (fun (o: a * s) => (id (fst o), snd o)) = id). {
+    apply functional_extensionality.
+    intro o; destruct o; reflexivity.
+  }
+  rewrite R1.
+  apply functor_identity.
+Qed.
 
 Lemma state_functor_composition_identity
       (m: Type -> Type)
@@ -210,7 +119,29 @@ Lemma state_functor_composition_identity
       (ps: StateT s m a)
   : state_map _ _ (u <<< v) ps == ((state_map _ _ u) <<< (state_map _ _ v)) ps.
 Proof.
-Admitted.
+  cbn.
+  unfold function_weq, state_map.
+  intros x.
+  assert (R1: (fun o : a * s => ((v >>> u) (fst o), snd o))
+              = ((fun o : b * s => (v (fst o), snd o))
+                   >>> (fun o : a * s => (u (fst o), snd o)))). {
+    apply functional_extensionality.
+    intros y.
+    destruct y.
+    cbn.
+    assert (R2: ((fun o : b * s => (v (fst o), snd o)) >>> (fun o : a * s => (u (fst o), snd o)))
+                = (fun o => ((v >>> u) (fst o), snd o))). {
+      apply functional_extensionality.
+      intros z.
+      destruct z.
+      reflexivity.
+    }
+    rewrite R2.
+    reflexivity.
+  }
+  rewrite R1.
+  apply functor_composition_identity.
+Qed.
 
 Instance state_Functor
          (m: Type -> Type)
@@ -233,36 +164,177 @@ Definition state_apply
            (f:   StateT s m (a -> b))
            (fs:  StateT s m a)
   : StateT s m b :=
-  fun s
-  => u <- f s                                                       ;
+  fun x
+  => u <- f x                                                       ;
      v <- fs (snd u)                                                ;
      pure ((fst u) (fst v), snd v).
 
-Lemma state_apply_composition
+Definition state_pure
+           {m: Type -> Type}
+          `{Monad m}
+           {s: Type}
+           (a: Type)
+           (x: a)
+  : StateT s m a :=
+  fun t => pure (x, t).
+
+Lemma state_applicative_identity
+      {m: Type -> Type}
+     `{Monad m}
+      {s: Type}
+     `{WEq s}
+      {a : Type}
+     `{WEq a}
+      (v : StateT s m a):
+  state_apply _ _ (state_pure (a -> a) id) v == v.
+Proof.
+  cbn.
+  unfold function_weq, state_apply.
+  intros x.
+  assert (R1: (u <- state_pure (a -> a) id x; v0 <- v (snd u); pure (fst u (fst v0), snd v0))
+              == (v0 <- v x; pure (id (fst v0), snd v0))). {
+    cbn.
+    unfold function_weq, state_apply, state_pure, id.
+    rewrite monad_left_identity.
+    reflexivity.
+  }
+  rewrite R1.
+  unfold id.
+  assert (R2: (fun (v0: a * s) => pure (f:=m) (fst v0, snd v0))
+              = (fun v0 => pure v0)). {
+    apply functional_extensionality.
+    intro y.
+    destruct y.
+    reflexivity.
+  }
+  rewrite R2.
+  rewrite monad_right_identity.
+  reflexivity.
+Qed.
+
+Lemma state_applicative_homomorphism
+      {m: Type -> Type}
+     `{Monad m}
+      {s: Type}
+     `{WEq s}
+      {a b: Type}
+     `{WEq b}
+      (v: a -> b)
+      (x: a)
+  : state_apply _ _ (state_pure _ v) (state_pure _ x) == (state_pure _ (v x): StateT s m b).
+Proof.
+  cbn.
+  unfold function_weq, state_apply, state_pure.
+  intro y.
+  rewrite monad_left_identity.
+  cbn.
+  rewrite monad_left_identity.
+  cbn.
+  reflexivity.
+Qed.
+
+Lemma state_applicative_interchange
       (m: Type -> Type)
      `{Monad m}
       {s: Type}
      `{WEq s}
-      (a b c : Type)
-     `{WEq c}
-      (u: StateT s m (b -> c))
-      (v: StateT s m (a -> b))
-      (w : StateT s m a):
-  state_apply _ _ (state_apply _ _ (compose <$> u) v) w
-  == state_apply _ _ u (state_apply _ _ v w).
+      (a b : Type)
+     `{WEq b}
+      (u : StateT s m (a -> b))
+      (y : a)
+  : state_apply _ _ u (state_pure a y)
+    == state_apply _ _ (state_pure ((a -> b) -> b) (fun z : a -> b => z y)) u.
 Proof.
-Admitted.
+  cbn.
+  unfold function_weq.
+  intro x.
+  unfold state_apply, state_pure.
+  rewrite monad_left_identity.
+  cbn.
+  assert (R1: (fun (u0: ((a -> b) * s))
+               => (v <- pure (f:=m) (y, snd u0);
+                   pure (fst u0 (fst v), snd v)))
+             == (fun (v: ((a -> b) * s))
+                  => pure (f:=m) (fst v y, snd v))). {
+    cbn.
+    unfold function_weq.
+    intros z.
+    rewrite monad_left_identity.
+    reflexivity.
+  }
+  rewrite R1.
+  reflexivity.
+Qed.
 
-Instance state_Apply
+Instance state_Applicative
          (m: Type -> Type)
         `{Monad m}
          (s: Type)
         `{WEq s}
-  : Apply (StateT s m) :=
-  { apply := state_apply
+  : Applicative (StateT s m) :=
+  { pure := state_pure
+  ; apply := state_apply
   }.
 Proof.
-  + apply state_apply_composition.
+  + apply (@state_applicative_identity m H s H0).
+  + intros a b c C u v w.
+    cbn.
+    unfold function_weq, state_apply, state_pure.
+    intro x.
+    assert (R1: (u0 <- pure (@compose a b c, x); v0 <- u (snd u0); pure (fst u0 (fst v0), snd v0))
+                == (v0 <- u (snd (@compose a b c, x)); pure (fst (compose, x) (fst v0), snd v0))). {
+      rewrite monad_left_identity.
+      reflexivity.
+    }
+    repeat rewrite monad_bind_associativity.
+    rewrite monad_left_identity.
+    repeat rewrite monad_bind_associativity.
+    cbn.
+    assert (R2: (fun x0
+                 => (x1 <- pure (compose (fst x0), snd x0);
+                     u0 <- (v0 <- v (snd x1); pure (fst x1 (fst v0), snd v0));
+                     v0 <- w (snd u0); pure (fst u0 (fst v0), snd v0)))
+                == (fun u0
+                    => v0 <- (u1 <- v (snd u0); v0 <- w (snd u1); pure (fst u1 (fst v0), snd v0));
+                       pure (fst u0 (fst v0), snd v0))). {
+      intros y.
+      repeat rewrite monad_left_identity.
+      repeat rewrite monad_bind_associativity.
+      cbn.
+      assert (R3: (fun x0
+                  => (u0 <- pure (fst y >>> fst x0, snd x0);
+                      v0 <- w (snd u0); pure (fst u0 (fst v0), snd v0)))
+                  == fun x0
+                     => (v0 <- (v0 <- w (snd x0); pure (fst x0 (fst v0), snd v0));
+                         pure (fst y (fst v0), snd v0))). {
+        cbn.
+        intros z.
+        repeat rewrite monad_left_identity.
+        repeat rewrite monad_bind_associativity.
+        cbn.
+        assert (R4: (fun (v0: a * s)
+                     => pure (f:=m) ((fst y >>> fst z) (fst v0), snd v0))
+                    == (fun x0
+                        => v0 <- pure (fst z (fst x0), snd x0); pure (fst y (fst v0), snd v0))). {
+          cbn.
+          intros q.
+          repeat rewrite monad_left_identity.
+          cbn.
+          unfold compose.
+          reflexivity.
+        }
+        apply monad_bind_morphism.
+        intros n.
+        rewrite monad_left_identity.
+        reflexivity.
+      }
+      rewrite (monad_bind_morphism _ _ _ R3).
+      reflexivity.
+    }
+    rewrite (monad_bind_morphism _ _ _ R2).
+    reflexivity.
+  + apply (@state_applicative_homomorphism m H s H0).
+  + apply (@state_applicative_interchange m H s H0).
 Defined.
 
 Definition state_bind
@@ -290,122 +362,12 @@ Lemma state_bind_associativity
   : state_bind b c (state_bind a b f g) h
     == state_bind a c f (fun x : a => state_bind b c (g x) h).
 Proof.
-Admitted.
-
-Instance state_Bind
-         (m: Type -> Type)
-        `{Monad m}
-         (s: Type)
-        `{WEq s}
-  : Bind (StateT s m) :=
-  { bind := state_bind
-  }.
-Proof.
-  + apply state_bind_associativity.
-Defined.
-
-Definition state_pure
-           {m: Type -> Type}
-          `{Monad m}
-           {s: Type}
-           (a: Type)
-           (x: a)
-  : StateT s m a :=
-  fun t => pure (x, t).
-
-Lemma state_applicative_identity
-      {m: Type -> Type}
-     `{Monad m}
-      {s: Type}
-     `{WEq s}
-      {a : Type}
-     `{WEq a}
-      (v : StateT s m a):
-  state_pure (a -> a) id <*> v == v.
-Proof.
-Admitted.
-
-Lemma state_applicative_composition
-      {m: Type -> Type}
-     `{Monad m}
-      {s: Type}
-     `{WEq s}
-      {a b c : Type}
-     `{WEq c}
-      (u : StateT s m (b -> c))
-      (v : StateT s m (a -> b))
-      (w : StateT s m a)
-  : state_pure ((b -> c) -> (a -> b) -> a -> c) compose <*> u <*> v <*> w
-    == u <*> (v <*> w).
-Proof.
-Admitted.
-
-Lemma state_applicative_homomorphism
-      {m: Type -> Type}
-     `{Monad m}
-      {s: Type}
-     `{WEq s}
-      {a b: Type}
-     `{WEq b}
-      (v: a -> b)
-      (x: a)
-  : state_pure _ v <*> state_pure _ x == (state_pure _ (v x): StateT s m b).
-Proof.
-Admitted.
-
-Lemma state_applicative_interchange
-      (m: Type -> Type)
-     `{Monad m}
-      {s: Type}
-     `{WEq s}
-      (a b : Type)
-     `{WEq b}
-      (u : StateT s m (a -> b))
-      (y : a)
-  : u <*> state_pure a y
-    == state_pure ((a -> b) -> b) (fun z : a -> b => z y) <*> u.
-Proof.
-Admitted.
-
-Instance state_Applicative
-         (m: Type -> Type)
-        `{Monad m}
-         (s: Type)
-        `{WEq s}
-  : Applicative (StateT s m) :=
-  { pure := state_pure
-  }.
-Proof.
-  + apply (@state_applicative_identity m H s H0).
-  + apply (@state_applicative_composition m H s H0).
-  + apply (@state_applicative_homomorphism m H s H0).
-  + apply (@state_applicative_interchange m H s H0).
-Defined.
-
-Lemma state_monad_left_identity
-      (m: Type -> Type)
-     `{Monad m}
-      {s: Type}
-     `{WEq s}
-      (a b : Type)
-     `{WEq b}
-      (x : a)
-      (f : a -> StateT s m b)
-  : (a <- pure x; f a) == f x.
-Proof.
-Admitted.
-
-Lemma state_monad_right_identity
-      (m: Type -> Type)
-     `{Monad m}
-      {s: Type}
-     `{WEq s}
-      (a : Type)
-     `{WEq a}
-      (x : StateT s m a)
-  : (y <- x; pure y) == x.
-Proof.
-Admitted.
+  cbn.
+  unfold state_bind, function_weq.
+  intros x.
+  rewrite monad_bind_associativity.
+  reflexivity.
+Qed.
 
 Instance state_Monad
          (m: Type -> Type)
@@ -413,11 +375,40 @@ Instance state_Monad
          (s: Type)
         `{WEq s}
   : Monad (StateT s m) :=
-  {
+  { bind := state_bind
   }.
 Proof.
-  + apply state_monad_left_identity.
-  + apply state_monad_right_identity.
+  + intros a b B x f.
+    cbn.
+    unfold function_weq, state_bind, state_pure.
+    intros y.
+    rewrite monad_left_identity.
+    reflexivity.
+  + intros a A x.
+    cbn.
+    unfold function_weq, state_bind, state_pure.
+    intros y.
+    assert (R1: (fun (u: (a * s)) => pure (f:=m) (fst u, snd u))
+                = fun (u: (a * s)) => pure u). {
+      apply functional_extensionality.
+      intros [z  z'].
+      reflexivity.
+    }
+    rewrite R1.
+    apply monad_right_identity.
+  + apply state_bind_associativity.
+  + intros a b B p f f' Heq.
+    cbn.
+    unfold function_weq, state_bind.
+    intros x.
+    assert (R1: (fun u => f (fst u) (snd u))
+                == fun u => f' (fst u) (snd u)). {
+      cbn.
+      intros y.
+    apply Heq.
+    }
+    rewrite (monad_bind_morphism _ _ _ R1).
+    reflexivity.
 Defined.
 
 Definition state_lift
